msl_application/GraphBi_Copy.v
@@ -55,7 +55,7 @@ Global Existing Instance CCS.
 
 Definition empty_Graph: Graph := empty_Graph null (null, L).
 
-Definition initial_copied_Graph (x x0: addr) (g: Graph): LGraph := single_vertex_labeledgraph (LocalGraphCopy.vmap (Graph_gen g x x0) x) null (null, L).
+Definition initial_copied_Graph (x x0: addr) (g: Graph): LGraph := single_vertex_labeledgraph (LocalGraphCopy.vmap (Graph_vgen g x x0) x) null (null, L).
 
 Opaque empty_Graph initial_copied_Graph.
 
@@ -74,6 +74,19 @@ Proof.
   subst; congruence.
 Qed.
 
+Lemma vmap_weaken: forall (g1 g2: Graph) x x0 BLA,
+  (x = null /\ x0 = null \/ x0 = BLA) ->
+  (~ vvalid g1 x /\ ~ vvalid g2 x0 \/ x0 = BLA).
+Proof.
+  intros.
+  destruct H; [left | right]; auto.
+  destruct H.
+  pose proof (@valid_not_null _ _ _ _ g1 _ (maGraph g1) x).
+  pose proof (@valid_not_null _ _ _ _ g2 _ (maGraph g2) x0).
+  unfold is_null_SGBA in *; simpl in *.
+  auto.
+Qed.
+
 Lemma root_stable_ramify: forall (g: Graph) (x: addr) (gx: addr * addr * addr),
   vgamma g x = gx ->
   vvalid g x ->
@@ -85,13 +98,13 @@ Proof. intros; apply va_reachable_root_stable_ramify; auto. Qed.
 
 Lemma root_update_ramify: forall (g: Graph) (x x0: addr) (lx: addr) (gx gx': addr * addr * addr) F,
   vgamma g x = gx ->
-  vgamma (Graph_gen g x lx) x = gx' ->
+  vgamma (Graph_vgen g x lx) x = gx' ->
   vvalid g x ->
   @derives pred _
     (F * reachable_vertices_at x g)
     (vertex_at x gx *
       (vertex_at x gx' -*
-       F * (vertices_at (fun u => vvalid (initial_copied_Graph x x0 g) u /\ x0 <> u) (initial_copied_Graph x x0 g) * reachable_vertices_at x (Graph_gen g x lx)))).
+       F * (vertices_at (fun u => vvalid (initial_copied_Graph x x0 g) u /\ x0 <> u) (initial_copied_Graph x x0 g) * reachable_vertices_at x (Graph_vgen g x lx)))).
 Proof.
   intros.
   rewrite !(sepcon_comm F).
@@ -114,7 +127,7 @@ Lemma not_null_copy1: forall (G: Graph) (x x0: addr) l r,
   vgamma G x = (null, l, r) ->
   vvalid G x ->
   x0 <> null ->
-  vcopy1 x G (Graph_gen G x x0) (initial_copied_Graph x x0 G) /\ x0 = LocalGraphCopy.vmap (Graph_gen G x x0) x.
+  vcopy1 x G (Graph_vgen G x x0) (initial_copied_Graph x x0 G) /\ x0 = LocalGraphCopy.vmap (Graph_vgen G x x0) x.
 Proof.
   intros.
   split; [split; [| split] |].
@@ -300,6 +313,119 @@ Proof.
       apply reachable_foot_valid in H6; auto.
 Qed.
 
+Lemma is_BiMaFin_disjoint_guard: forall (g1':  @LGraph pSGG_Bi (@addr pSGG_Bi) (prod (@addr pSGG_Bi) LR)) (g2'': Graph) x0 es0,
+  is_guarded_BiMaFin (fun v => x0 <> v) (fun e => ~ In e es0) g1' ->
+  vvalid g1' x0 ->
+  (forall e, In e es0 -> fst e = x0) ->
+  Disjoint addr (vvalid g2'') (vvalid g1') ->
+  disjointed_guard (vvalid g2'') (vvalid g1') (evalid g2'') (evalid g1').
+Proof.
+  intros.
+  split; auto.
+  rewrite Disjoint_spec in *.
+  intros e ? ?.
+  destruct (@valid_graph _ _ _ _ g2'' _ (maGraph _) e H3) as [? _].
+  apply (H2 _ H5).
+  destruct (in_dec equiv_dec e es0); destruct e as [v lr].
+  + specialize (H1 _ i).
+    simpl in H1.
+    rewrite left_right_sound0 by auto.
+    subst; auto.
+  + destruct H as [X _].
+    pose (pg1 := Build_GeneralGraph _ _ (fun g: LGraph => BiMaFin g) (gpredicate_sub_labeledgraph (fun v => x0 <> v) (fun e => ~ In e es0) g1') X: Graph).
+    assert (evalid pg1 (v, lr)) by (simpl; rewrite Intersection_spec; split; auto).
+    assert (src g2'' (v, lr) = src pg1 (v, lr)) by (rewrite !left_right_sound0; auto).
+    apply (@valid_graph _ _ _ _ pg1 _ (maGraph _)) in H.
+    destruct H as [? _].
+    rewrite H6; auto.
+    destruct H; auto.
+Qed.
+
+Lemma labeledgraph_add_edge_ecopy1_left: forall (g g1 g2: Graph) (g1' g2': LGraph) (x l r x0 l0: addr),
+  vvalid g x ->
+  vgamma g x = (null, l, r) ->
+  vcopy1 x g g1 g1' ->
+  extended_copy (dst g (x, L)) (g1: LGraph, g1') (g2: LGraph, g2') ->
+  x0 = LocalGraphCopy.vmap g1 x ->
+  l = null /\ l0 = null \/ l0 = LocalGraphCopy.vmap g2 l ->
+  let g3 := Graph_egen g2 (x, L) (x0, L): Graph in
+  let g3' := labeledgraph_add_edge g2' (x0, L) x0 l0 (null, L): LGraph in
+  ecopy1 (x, L) (g2: LGraph, g2') (g3: LGraph, g3').
+Proof.
+  intros.
+  unfold ecopy1.
+  split; [| split].
+  + reflexivity.
+  + apply WeakMarkGraph.labeledgraph_egen_do_nothing.
+  + destruct H4; [admit |].
+    pose proof LocalGraphCopy.labeledgraph_egen_ecopy1 g2 g2' (x, L) (x0, L).
+    rewrite !left_right_sound in H5 by admit.
+    replace (dst g2 (x, L)) with l in H5 by admit.
+    replace (@LocalGraphCopy.vmap (@addr pSGG_Bi)
+                  (prod (@addr pSGG_Bi) LR) (@addr pSGG_Bi)
+                  (prod (@addr pSGG_Bi) LR)
+                  (@SGBA_VE (@addr pSGG_Bi) (prod (@addr pSGG_Bi) LR)
+                     (@SGBA pSGG_Bi))
+                  (@SGBA_EE (@addr pSGG_Bi) (prod (@addr pSGG_Bi) LR)
+                     (@SGBA pSGG_Bi)) (@addr pSGG_Bi)
+                  (prod (@addr pSGG_Bi) LR) (@addr pSGG_Bi)
+                  (prod (@addr pSGG_Bi) LR)
+                  (@GMS (@addr pSGG_Bi) (prod (@addr pSGG_Bi) LR) CCS)
+                  (@Graph_LGraph pSGG_Bi (@addr pSGG_Bi)
+                     (prod (@addr pSGG_Bi) LR) g2) x)
+      with (@LocalGraphCopy.vmap (@addr pSGG_Bi)
+                  (prod (@addr pSGG_Bi) LR) (@addr pSGG_Bi)
+                  (prod (@addr pSGG_Bi) LR)
+                  (@SGBA_VE (@addr pSGG_Bi) (prod (@addr pSGG_Bi) LR)
+                     (@SGBA pSGG_Bi))
+                  (@SGBA_EE (@addr pSGG_Bi) (prod (@addr pSGG_Bi) LR)
+                     (@SGBA pSGG_Bi)) (@addr pSGG_Bi)
+                  (prod (@addr pSGG_Bi) LR) (@addr pSGG_Bi)
+                  (prod (@addr pSGG_Bi) LR)
+                  (@GMS (@addr pSGG_Bi) (prod (@addr pSGG_Bi) LR) CCS)
+                  (@Graph_LGraph pSGG_Bi (@addr pSGG_Bi)
+                     (prod (@addr pSGG_Bi) LR) g1) x) in H5 by admit.
+    rewrite <- H3, <- H4 in H5.
+    apply H5.
+split; [| split; [| split; [| split; [| split; [| split]]]]].
+    - reflexivity.
+    - intros v; reflexivity.
+    - rewrite guarded_pointwise_relation_spec; intros.
+      simpl.
+      unfold update_elabel; simpl.
+      destruct_eq_dec (x, L) x1; auto.
+      unfold Complement, Ensembles.In in H6; congruence.
+    - intros.
+      simpl.
+      unfold update_elabel.
+      destruct_eq_dec (x, L) (x, L); [| congruence].
+      destruct_eq_dec (x, L) e0; auto.
+      change (elabel (lg_gg g2) e0) with (LocalGraphCopy.emap g2 e0).
+      (* assert (evalid g2' (LocalGraphCopy.emap g2 e0)); [| intro HH; rewrite HH in *; tauto]. *)
+      Print LocalGraphCopy.ecopy1.
+      admit.
+    - split; [| split; [| split]]; simpl.
+      * apply Prop_join_Empty.
+      * unfold update_elabel, add_evalid; simpl.
+        destruct_eq_dec (x, L) (x, L); [| congruence].
+        apply Prop_join_x1.
+        admit.
+      * unfold update_src, add_evalid; simpl.
+        intros. admit.
+      * admit.
+    - simpl.
+      unfold update_src, update_elabel; simpl.
+      destruct_eq_dec (x, L) (x, L); [| congruence].
+      destruct_eq_dec (x0, L) (x0, L); [| congruence].
+      admit.
+    - simpl.
+      unfold update_dst, update_elabel; simpl.
+      destruct_eq_dec (x, L) (x, L); [| congruence].
+      destruct_eq_dec (x0, L) (x0, L); [| congruence].
+      admit.
+Qed.
+
+
 Lemma extend_copy_left: forall (g g1 g2: Graph) (g1': LGraph) (g2'': Graph) (x l r x0 l0: addr) d0,
   vvalid g x ->
   vgamma g x = (null, l, r) ->
@@ -307,15 +433,18 @@ Lemma extend_copy_left: forall (g g1 g2: Graph) (g1': LGraph) (g2'': Graph) (x l
   copy l g1 g2 g2'' ->
   x0 = LocalGraphCopy.vmap g1 x ->
   l = null /\ l0 = null \/ l0 = LocalGraphCopy.vmap g2 l ->
+  is_guarded_BiMaFin (fun v => x0 <> v) (fun e => ~ In e nil) g1' ->
+  let g3 := Graph_egen g2 (x, L) (x0, L): Graph in
   @derives pred _
   (vertex_at x0 d0 * vertices_at (fun x => vvalid g1' x /\ x0 <> x) g1' * reachable_vertices_at l0 g2'') 
-  (EX g2': LGraph,
-    !! edge_copy g (x, L) (g1: LGraph, g1') (g2: LGraph, g2') && 
-    vertex_at x0 d0 * vertices_at (fun x => vvalid g2' x /\ x0 <> x) g2').
+  (EX g3': LGraph,
+    !! (edge_copy g (x, L) (g1: LGraph, g1') (g3: LGraph, g3') /\ is_guarded_BiMaFin (fun v => x0 <> v) (fun e => ~ In e ((x0, L) :: nil)) g3') && 
+    (vertex_at x0 d0 * vertices_at (fun x => vvalid g3' x /\ x0 <> x) g3')).
 Proof.
   intros.
+  rename H5 into BMF.
   inversion H0.
-  pose proof vcopy1_edge_copy_list_copy_extended_copy x ((x, L) :: (x, R) :: nil) nil (x, L) ((x, R) :: nil) g g1 g1 g1' g1' g2 g2'' l l0 H.
+  pose proof @vcopy1_edge_copy_list_weak_copy_extended_copy _ _ _ _ _ BiMaFin_Normal x ((x, L) :: (x, R) :: nil) nil (x, L) ((x, R) :: nil) g g1 g1 g1' g1' g2 g2'' l l0 H.
   spec H5; [simpl; unfold Complement, Ensembles.In; congruence |].
   spec H5; [reflexivity |].
   spec H5; [intros; apply (biGraph_out_edges g (biGraph _)); auto |].
@@ -324,6 +453,7 @@ Proof.
   spec H5; [hnf; auto |].
   spec H5; [auto |].
   spec H5; [subst l; auto |].
+
   unfold reachable_vertices_at.
   pose proof vertices_at_sepcon_unique_1x (Graph_SpatialGraph g2'') x0 (reachable g2'' l0) d0.
   pose proof vertices_at_sepcon_unique_xx g1' (Graph_SpatialGraph g2'') (fun x1 : addr => vvalid g1' x1 /\ x0 <> x1) (reachable g2'' l0).
@@ -332,16 +462,30 @@ Proof.
   clear H9 H10.
   spec H5.
   Focus 1. {
-    split.
+    apply is_BiMaFin_disjoint_guard with (x0 := x0) (es0 := nil); auto.
+    + destruct H1 as [_ [_ ?]].
+      destruct H1 as [_ [_ [_ ?]]].
+      subst g1' x0.
+      simpl; auto.
+    + intros ? [].
     + destruct H2 as [? [? ?]].
-      rewrite (LocalGraphCopy.copy_vvalid_eq _ _ _ _ _ H10).
-      rewrite Disjoint_spec in H11 |- *.
-      destruct H4.
-      clear - H11 H12; intros x1.
-      specialize (H11 x1).
-      destruct_eq_dec x0 x1.
-      - subst.
-Admitted.
+      apply (vmap_weaken g1 g2'') in H4.
+      rewrite (LocalGraphCopy.copy_vvalid_weak_eq g1 g2 g2'' (WeakMarkGraph.marked g1) l l0 H4 H10).
+      apply Disjoint_comm.
+      apply (Disjoint_x1 _ _ _ H11 H12).
+  } Unfocus.
+
+  unfold map in H5; rewrite H3 in BMF.
+  specialize (H5 BMF).
+  specialize (H5 (Graph_is_BiMaFin _)).
+
+  destruct H5 as [g2' [? [? [? ?]]]].
+  pose (g3' := labeledgraph_add_edge g2' (x0, L) x0 l0 (null, L) : LGraph).
+  apply (exp_right g3').
+  apply andp_right; [apply prop_right; split | rewrite sepcon_assoc; apply sepcon_derives; auto].
+  + unfold edge_copy.
+    split_relation_list ((g2: LGraph, g2' : LGraph) :: nil); auto.
+    
 (*
   intros.
   pose proof WeakMarkGraph.triple_mark1 x g g g1 as HH1.
